src/program_proof/simplepb/simplelog/proof.v
@@ -1,0 +1,229 @@
+From Perennial.program_proof Require Import grove_prelude.
+From Goose.github_com.mit_pdos.gokv.simplepb Require Export simplelog.
+From Perennial.program_proof Require Import marshal_stateless_proof.
+From coqutil.Datatypes Require Import List.
+
+From Perennial.program_proof.aof Require Import proof.
+
+Section proof.
+
+(* State machine definition *)
+Record SMRecord :=
+  {
+    sm_OpType:Type ;
+    sm_has_op_encoding : list u8 → sm_OpType → Prop ;
+    sm_has_snap_encoding: list u8 → (list sm_OpType) → Prop ;
+    sm_has_op_encoding_injective : ∀ o1 o2 l, sm_has_op_encoding l o1 → sm_has_op_encoding l o2 → o1 = o2 ;
+    sm_compute_reply : list sm_OpType → sm_OpType → list u8 ;
+  }.
+
+Context {sm_record:SMRecord}.
+Notation OpType := (sm_OpType sm_record).
+Notation has_op_encoding := (sm_has_op_encoding sm_record).
+Notation has_snap_encoding := (sm_has_snap_encoding sm_record).
+Notation has_op_encoding_injective := (sm_has_op_encoding_injective sm_record).
+Notation compute_reply := (sm_compute_reply sm_record).
+
+Context `{!heapGS Σ}.
+Context `{!aofG Σ}.
+
+(* Want to prove *)
+
+Definition file_encodes_state (data:list u8) (epoch:u64) (ops: list OpType) (sealed:bool): Prop.
+Admitted.
+
+Lemma file_encodes_state_inj data e ops s e' ops' s':
+  file_encodes_state data e ops s →
+  file_encodes_state data e' ops' s' →
+  e = e' ∧
+  ops = ops' ∧
+  s = s'.
+Proof.
+Admitted.
+
+Lemma file_encodes_state_append op op_bytes data epoch ops :
+  has_op_encoding op_bytes op →
+  file_encodes_state data epoch ops false →
+  file_encodes_state (data ++ (u64_le (length op_bytes)) ++ op_bytes) epoch (ops++[op]) false
+.
+Proof.
+Admitted.
+
+Implicit Types (P:u64 → list OpType → bool → iProp Σ).
+
+Definition file_inv P (contents:list u8) : iProp Σ :=
+  ∃ epoch ops sealed,
+  ⌜file_encodes_state contents epoch ops sealed⌝ ∗
+  P epoch ops sealed
+.
+
+Implicit Types own_InMemoryStateMachine : list OpType → iProp Σ.
+
+Definition is_InMemory_applyVolatileFn (applyVolatileFn:val) own_InMemoryStateMachine : iProp Σ :=
+  ∀ ops op op_sl op_bytes,
+  {{{
+        ⌜has_op_encoding op_bytes op⌝ ∗
+        readonly (is_slice_small op_sl byteT 1 op_bytes) ∗
+        own_InMemoryStateMachine ops
+  }}}
+    applyVolatileFn (slice_val op_sl)
+  {{{
+        reply_sl q, RET (slice_val reply_sl);
+        own_InMemoryStateMachine (ops ++ [op]) ∗
+        is_slice_small reply_sl byteT q (compute_reply ops op)
+  }}}
+.
+
+Definition is_InMemoryStateMachine (sm:loc) own_InMemoryStateMachine : iProp Σ :=
+  ∃ applyVolatileFn,
+  "#HapplyVolatile" ∷ readonly (sm ↦[InMemoryStateMachine :: "ApplyVolatile"] applyVolatileFn) ∗
+  "#HapplyVolatile_spec" ∷ is_InMemory_applyVolatileFn applyVolatileFn own_InMemoryStateMachine
+.
+
+Definition own_StateMachine γaof (s:loc) (epoch:u64) (ops:list OpType) (sealed:bool) P : iProp Σ :=
+  ∃ (fname:string) (aof_ptr:loc) (logsize:u64) (smMem_ptr:loc) data
+    own_InMemoryStateMachine,
+    "Hfname" ∷ s ↦[StateMachine :: "fname"] #(LitString fname) ∗
+    "HlogFile" ∷ s ↦[StateMachine :: "logFile"] #aof_ptr ∗
+    "HsmMem" ∷ s ↦[StateMachine :: "smMem"] #smMem_ptr ∗
+    "HnextIndex" ∷ s ↦[StateMachine :: "nextIndex"] #(U64 (length ops)) ∗
+    "Hlogsize" ∷ s ↦[StateMachine :: "logsize"] #logsize ∗
+
+    "Haof" ∷ aof_log_own γaof data ∗
+    "#His_aof" ∷ is_aof aof_ptr γaof fname (file_inv P) ∗
+    "%Henc" ∷ ⌜file_encodes_state data epoch ops sealed⌝ ∗
+    "Hmemstate" ∷ own_InMemoryStateMachine ops ∗
+    "#HisMemSm" ∷ is_InMemoryStateMachine smMem_ptr own_InMemoryStateMachine
+    (* "HsmMem" ∷ *)
+.
+
+Lemma StateMachine__apply s Q (op:OpType) (op_bytes:list u8) op_sl γaof epoch ops P :
+  {{{
+        ⌜has_op_encoding op_bytes op⌝ ∗
+        readonly (is_slice_small op_sl byteT 1 op_bytes) ∗
+        (P epoch ops false ={⊤}=∗ P epoch (ops ++ [op]) false ∗ Q) ∗
+        own_StateMachine γaof s epoch ops false P
+  }}}
+    StateMachine__apply #s (slice_val op_sl)
+  {{{
+        reply_sl q (waitFn:goose_lang.val),
+        RET (slice_val reply_sl, waitFn);
+        is_slice_small reply_sl byteT q (compute_reply ops op) ∗
+        own_StateMachine γaof s epoch (ops ++ [op]) false P ∗
+        (∀ Ψ, (Q -∗ Ψ #()) -∗ WP waitFn #() {{ Ψ }})
+  }}}
+.
+Proof.
+  iIntros (Φ) "(%HopEnc & #Hop_sl & Hupd & Hown) HΦ".
+  wp_lam.
+  wp_pures.
+
+  iNamed "Hown".
+
+  (* first, apply the operation in memory and to compute the reply *)
+  iAssert (_) with "HisMemSm" as "#HisMemSm2".
+  iNamed "HisMemSm2".
+  wp_loadField.
+  wp_loadField.
+  wp_apply ("HapplyVolatile_spec" with "[$Hmemstate]").
+  {
+    iFrame "#".
+    done.
+  }
+  iIntros (??) "[Hmemstate Hreply_sl]".
+  wp_pures.
+
+  wp_loadField.
+  wp_storeField.
+  wp_loadField.
+  wp_apply (wp_slice_len).
+  wp_storeField.
+
+  wp_loadField.
+  wp_if_destruct.
+  {
+    admit. (* TODO: get rid of this panic *)
+  }
+
+  (* make opWithLen *)
+  iMod (readonly_load with "Hop_sl") as (?) "Hop_sl2".
+  iDestruct (is_slice_small_sz with "Hop_sl2") as %Hop_sz.
+  wp_apply (wp_slice_len).
+  wp_apply (wp_NewSliceWithCap).
+  { apply encoding.unsigned_64_nonneg. }
+  iIntros (?) "HopWithLen_sl".
+  wp_apply (wp_ref_to).
+  { done. }
+  iIntros (opWithLen_sl_ptr) "HopWithLen".
+  wp_pures.
+  wp_apply wp_slice_len.
+  wp_load.
+  wp_apply (wp_WriteInt with "[$HopWithLen_sl]").
+  iIntros (opWithLen_sl) "HopWithLen_sl".
+  wp_store.
+  wp_load.
+  wp_apply (wp_WriteBytes with "[$HopWithLen_sl $Hop_sl2]").
+  rename opWithLen_sl into opWithLen_sl_old.
+  iIntros (opWithLen_sl) "[HopWithLen_sl _]".
+  wp_store.
+
+  (* start append on logfile *)
+  wp_load.
+  wp_loadField.
+
+  iDestruct (is_slice_to_small with "HopWithLen_sl") as "HopWithLen_sl".
+
+  (* simplify marshalled opWithLen list *)
+  replace (int.nat 0) with (0%nat) by word.
+  rewrite replicate_0.
+  rewrite app_nil_l.
+  replace (op_sl.(Slice.sz)) with (U64 (length op_bytes)); last first.
+  { word. }
+
+  wp_apply (wp_AppendOnlyFile__Append with "His_aof [$Haof $HopWithLen_sl Hupd]").
+  { rewrite app_length. rewrite u64_le_length. word. }
+  { admit. } (* TODO: list size overflow *)
+  {
+    instantiate (1:=Q).
+    iIntros "Hi".
+    iDestruct "Hi" as (???) "[%Henc2 HP]".
+    pose proof (file_encodes_state_inj _ _ _ _ _ _ _ Henc2 Henc) as [-> [-> ->]].
+    iMod ("Hupd" with "HP") as "[HP $]".
+    iModIntro.
+    iExists _, (ops ++ [op]), _.
+    iFrame "HP".
+    iPureIntro.
+    by apply file_encodes_state_append.
+  }
+  iIntros (l) "[Haof HupdQ]".
+  wp_pures.
+  wp_loadField.
+  wp_pures.
+  iModIntro.
+  iApply "HΦ".
+  iFrame.
+  iSplitR "HupdQ".
+  {
+    iExists _, _, _, _, _, _.
+    iFrame "∗#".
+    iSplitL; last first.
+    { iPureIntro. by apply file_encodes_state_append. }
+    iApply to_named.
+    iExactEq "HnextIndex".
+    repeat f_equal.
+    rewrite app_length.
+    simpl.
+    admit. (* TODO: show that the length of the ops list does not overflow *)
+  }
+  iIntros (Ψ) "HΨ".
+  wp_call.
+  wp_apply (wp_AppendOnlyFile__WaitAppend with "[$His_aof]").
+  iIntros "Haof_len".
+  iMod ("HupdQ" with "Haof_len") as "HQ".
+  wp_pures.
+  iModIntro.
+  iApply "HΨ".
+  iFrame.
+Admitted.
+
+End proof.
